proved X;X equals to I

theories/transform/Transform.v
@@ -21,13 +21,17 @@ Section Transform.
 
 Variable nq: nat.
 
+(* Qbit index validity : prevents index out of bounds *)
+Definition Qbit_index_valid (qbit: nat): Prop :=
+  nq > qbit.
+
 Lemma Transform_I: forall (qbit: nat),
-  Instruction_equivalence nq
+  Instruction_equiv nq
   (Gate_I qbit)
   NopInstr.
 Proof.
   intros qbit.
-  unfold Instruction_equivalence, ProgramState_equivalence.
+  unfold Instruction_equiv, ProgramState_equiv.
   intros ps Hinv.
   unfold PositiveMap.Equal.
   intros cstate.
@@ -37,35 +41,38 @@ Qed.
 
 Lemma Transform_X_X_Branch:
   forall (b: Branch nq) (qbit: nat),
+  Qbit_index_valid qbit ->
   b = Execute_rotate_instr_branch nq PI 0 PI qbit (Execute_rotate_instr_branch nq PI 0 PI qbit b).
 Proof.
-  intros b qbit.
+  intros b qbit H.
   unfold Execute_rotate_instr_branch.
   destruct b eqn:Hb.
   simpl.
   f_equal.
-  remember (mat_single nq qbit (mat_rot PI 0 PI)) as A.
-  assert (Hu: mat_unitary A).
-  {
-    rewrite HeqA. apply mat_single_unitary. apply mat_rot_unitary.
-  }
-  (* Problem: A is not Hermitian due to the global phase *)
+  change (mat_single nq qbit (mat_rot PI 0 PI)) with (Gate_X_matrix nq qbit).
+  remember (Gate_X_matrix nq qbit) as A.
   unfold den_uop.
-  rewrite (mat_mul_assoc A _ _), (mat_mul_assoc A _ _).
-  rewrite <- HH at 2. rewrite HH at 2.
-  rewrite (proj2 Hu), mat_mul_eye_l, <- mat_mul_assoc.
-  rewrite (proj2 Hu), mat_mul_eye_r.
-  reflexivity.
-Admitted.
+  rewrite (mat_mul_assoc A _ _), (mat_mul_assoc A _ _), <- (mat_mul_assoc _ (A†) (A†)).
+  rewrite <- mat_mul_conjtrans.
+  rewrite HeqA.
+  rewrite (Gate_X_matrix_square _ _ H).
+  rewrite mat_scale_conjtrans, mat_scale_mul_assoc, mat_mul_eye_l.
+  rewrite mat_scale_mul_comm, <- mat_scale_cmul_assoc, mat_eye_conjtrans.
+  rewrite <- mat_scale_mul_comm, mat_mul_eye_r.
+  com_simpl.
+  assert (Hcom: ((-1)%R * (-1)%R = Cone)%com). unfold com_mul, Cone. simpl. f_equal. lra. lra.
+  rewrite Hcom, mat_scale_1. reflexivity. 
+Qed.
 
 Lemma Transform_X_X: forall (qbit: nat),
-  Instruction_equivalence nq
+  Qbit_index_valid qbit ->
+  Instruction_equiv nq
   (SeqInstr (Gate_X qbit) (Gate_X qbit))
   (Gate_I qbit).
 Proof.
   intros qbit.
-  unfold Instruction_equivalence, ProgramState_equivalence.
-  intros ps Hinv.
+  unfold Instruction_equiv, ProgramState_equiv.
+  intros H ps Hinv.
   unfold PositiveMap.Equal.
   intros cstate. simpl.
   destruct (PositiveMap.find cstate ps) eqn:Hfind.
@@ -75,7 +82,7 @@ Proof.
     apply PositiveMap.map_1 with (f:=Execute_rotate_instr_branch nq PI 0 PI qbit) in Hfind.
     apply PositiveMap.map_1 with (f:=Execute_rotate_instr_branch nq PI 0 PI qbit) in Hfind.
     remember (Execute_rotate_instr_branch nq PI 0 PI qbit (Execute_rotate_instr_branch nq PI 0 PI qbit b)) as b'.
-    rewrite <- Transform_X_X_Branch in Heqb'.
+    rewrite <- (Transform_X_X_Branch _ _ H) in Heqb'.
     rewrite <- Heqb'.
     apply Hfind.
   - unfold Execute_rotate_instr.
